Organized the tests
- Replaced the outdated Move stdlibs with new ones
- Deleted the legacy mvir test files which have been ported, so no longer necessary
- Added more test cases (porting some leftovers)
- Added README.md in the test folder `move-prover/tests`
- Updated the commands in `scripts/README.md` to set the env variables
  properly

Closes: #3282
Approved by: wrwg

language/move-prover/tests/sources/hash_model.move
@@ -4,7 +4,9 @@ module TestHash {
 
     use 0x0::Hash;
 
-    // sha2 tests
+    // -----------
+    // SHA-2 Tests
+    // -----------
 
     fun hash_test1(v1: vector<u8>, v2: vector<u8>): (vector<u8>, vector<u8>)
     {
@@ -32,7 +34,23 @@ module TestHash {
         ensures result == (v1 == v2);
     }
 
-    // sha3 tests
+    fun hash_test1_incorrect(v1: vector<u8>, v2: vector<u8>): (vector<u8>, vector<u8>)
+    {
+        let h1 = Hash::sha2_256(v1);
+        let h2 = Hash::sha2_256(v2);
+        (h1, h2)
+    }
+    spec fun hash_test1_incorrect {
+        aborts_if false;
+        // ensures result_1 == result_2; // TODO: uncomment this after fixing the non-determinism issue of Boogie
+        ensures len(result_1) > 0 ==> result_1[0] < max_u8(); // should be <=
+    }
+
+
+    // -----------
+    // SHA-3 Tests
+    // -----------
+
     fun hash_test3(v1: vector<u8>, v2: vector<u8>): (vector<u8>, vector<u8>)
     {
         let h1 = Hash::sha3_256(v1);
@@ -57,5 +75,17 @@ module TestHash {
     spec fun hash_test4 {
         aborts_if false;
         ensures result == (v1 == v2);
+    }
+
+    fun hash_test2_incorrect(v1: vector<u8>, v2: vector<u8>): (vector<u8>, vector<u8>)
+    {
+        let h1 = Hash::sha3_256(v1);
+        let h2 = Hash::sha3_256(v2);
+        (h1, h2)
+    }
+    spec fun hash_test2_incorrect {
+        aborts_if false;
+        // ensures result_1 == result_2; // TODO: uncomment this after fixing the non-determinism issue of Boogie
+        ensures len(result_1) > 0 ==> result_1[0] < max_u8();
     }
 }
