language/move-prover/tests/sources/resources.move
@@ -3,6 +3,10 @@
 module TestResources {
     use 0x0::Transaction;
 
+    // ---------------
+    // Simple resource
+    // ---------------
+
     resource struct R {
         x: u64
     }
@@ -15,13 +19,159 @@ module TestResources {
         ensures exists<R>(sender());
     }
 
-    fun create_resource_bad() {
+    fun create_resource_incorrect() {
         if(exists<R>(Transaction::sender())) {
             abort 1
         };
     }
-    spec fun create_resource_bad {
+    spec fun create_resource_incorrect {
         aborts_if exists<R>(sender());
         ensures exists<R>(sender());
+    }
+
+    fun move_from_addr(a: address) acquires R {
+        let r = move_from<R>(a);
+        let R{x: _} = r;
+    }
+    spec fun move_from_addr {
+        aborts_if !exists<R>(a);
+    }
+
+    fun move_from_addr_to_sender(a: address) acquires R {
+        let r = move_from<R>(a);
+        let R{x: x} = r;
+        move_to_sender<R>(R{x: x});
+    }
+    spec fun move_from_addr_to_sender { // TODO: either a bug or an incomplete spec
+        //aborts_if !exists<R>(a);
+        //aborts_if exists<R>(sender());
+    }
+
+    fun borrow_global_mut_correct(a: address) acquires R {
+        let r = borrow_global_mut<R>(a);
+        _ = r;
+        let r2 = borrow_global_mut<R>(a);
+        _ = r2;
+    }
+    spec fun borrow_global_mut_correct {
+        aborts_if !exists<R>(a);
+    }
+
+
+    // ---------------
+    // Nested resource
+    // ---------------
+
+    resource struct A {
+        addr: address,
+        val: u64,
+    }
+
+    resource struct B {
+        val: u64,
+        a: A,
+    }
+
+    resource struct C {
+        val: u64,
+        b: B,
+    }
+
+    fun identity(a: A, b: B, c: C): (A,B,C) {
+        (a, b, c)
+    }
+    spec fun identity {
+        aborts_if false;
+        ensures result_1 == a;
+        ensures result_2 == b;
+        ensures result_3 == c;
+    }
+
+    fun pack_A(a: address, va: u64): A {
+        A{ addr:a, val:va }
+    }
+    spec fun pack_A {
+        aborts_if false;
+        ensures result.addr == a;
+        ensures result.val == va;
+    }
+
+    fun pack_B(a: address, va: u64, vb: u64): B {
+        let var_a = A{ addr: a, val: va };
+        let var_b = B{ val: vb, a: var_a };
+        var_b
+    }
+    spec fun pack_B {
+        aborts_if false;
+        ensures result.val == vb;
+        ensures result.a.val == va;
+        ensures result.a.addr == a;
+    }
+
+    fun pack_C(a: address, va: u64, vb: u64, vc: u64): C {
+        let var_a = A{ addr: a, val: va };
+        let var_b = B{ val: vb, a: var_a };
+        let var_c = C{ val: vc, b: var_b };
+        var_c
+    }
+    spec fun pack_C {
+        aborts_if false;
+        ensures result.val == vc;
+        ensures result.b.val == vb;
+        ensures result.b.a.val == va;
+        ensures result.b.a.addr == a;
+    }
+
+    fun unpack_A(a: address, va: u64): (address, u64) {
+        let var_a = A{ addr:a, val:va };
+        let A{addr: aa, val:v1} = var_a;
+        (aa, v1)
+    }
+    spec fun unpack_A {
+        aborts_if false;
+        ensures result_1 == a;
+        ensures result_2 == va;
+    }
+
+    fun unpack_B(a: address, va: u64, vb: u64): (address, u64, u64) {
+        let var_a = A{ addr: a, val: va };
+        let var_b = B{ val: vb, a: var_a };
+        let B{val: v2, a: A{ addr:aa, val: v1}} = var_b;
+        (aa, v1, v2)
+    }
+    spec fun unpack_B {
+        aborts_if false;
+        ensures result_1 == a;
+        ensures result_2 == va;
+        ensures result_3 == vb;
+    }
+
+    fun unpack_C(a: address, va: u64, vb: u64, vc: u64): (address, u64, u64, u64) {
+        let var_a = A{ addr: a, val: va };
+        let var_b = B{ val: vb, a: var_a };
+        let var_c = C{ val: vc, b: var_b };
+        let C{val: v3, b: B{val: v2, a: A{ addr:aa, val: v1}}} = var_c;
+        (aa, v1, v2, v3)
+    }
+    spec fun unpack_C {
+        aborts_if false;
+        ensures result_1 == a;
+        ensures result_2 == va;
+        ensures result_3 == vb;
+        ensures result_4 == vc;
+    }
+
+    fun ref_A(a: address, b: bool): A {
+        let var_a = if (b) A{ addr: a, val: 1 }
+                    else A{ addr: a, val: 42 };
+        let var_a_ref = &var_a;
+        let b_val_ref = &var_a_ref.val;
+        let b_var = *b_val_ref;
+        if (b_var != 42) abort 42;
+        var_a
+    }
+    spec fun ref_A {
+        aborts_if b;
+        ensures result.addr == a;
     }
 }
