language/move-prover/tests/sources/stdlib/modules/script_whitelist.move
@@ -1,0 +1,28 @@
+// dep: tests/sources/stdlib/modules/libra_configs.move
+// dep: tests/sources/stdlib/modules/transaction.move
+// dep: tests/sources/stdlib/modules/libra_system.move
+// dep: tests/sources/stdlib/modules/libra_account.move
+// dep: tests/sources/stdlib/modules/hash.move
+// dep: tests/sources/stdlib/modules/lbr.move
+// dep: tests/sources/stdlib/modules/lcs.move
+// dep: tests/sources/stdlib/modules/libra.move
+// dep: tests/sources/stdlib/modules/libra_transaction_timeout.move
+// dep: tests/sources/stdlib/modules/vector.move
+// dep: tests/sources/stdlib/modules/libra_time.move
+// dep: tests/sources/stdlib/modules/validator_config.move
+
+address 0x0:
+
+module ScriptWhitelist {
+    use 0x0::LibraConfig;
+
+    struct T { payload: vector<u8> }
+
+    public fun initialize(payload: vector<u8>) {
+        LibraConfig::publish_new_config<Self::T>(T { payload })
+    }
+
+    public fun set(payload: vector<u8>) {
+        LibraConfig::set<Self::T>(T { payload } )
+    }
+}
