language/move-prover/tests/sources/stdlib/modules/transaction_fee.move
@@ -1,23 +1,21 @@
 // dep: tests/sources/stdlib/modules/libra_account.move
-// dep: tests/sources/stdlib/modules/libra_system.move
-// dep: tests/sources/stdlib/modules/address_util.move
+// dep: tests/sources/stdlib/modules/hash.move
+// dep: tests/sources/stdlib/modules/lbr.move
+// dep: tests/sources/stdlib/modules/lcs.move
+// dep: tests/sources/stdlib/modules/libra.move
+// dep: tests/sources/stdlib/modules/libra_transaction_timeout.move
 // dep: tests/sources/stdlib/modules/transaction.move
 // dep: tests/sources/stdlib/modules/vector.move
-// dep: tests/sources/stdlib/modules/libra_coin.move
-// dep: tests/sources/stdlib/modules/validator_config.move
-// dep: tests/sources/stdlib/modules/u64_util.move
-// dep: tests/sources/stdlib/modules/hash.move
 // dep: tests/sources/stdlib/modules/libra_time.move
-// dep: tests/sources/stdlib/modules/libra_transaction_timeout.move
-// no-verify
+// dep: tests/sources/stdlib/modules/libra_system.move
+// dep: tests/sources/stdlib/modules/validator_config.move
+
 address 0x0:
 
 module TransactionFee {
     use 0x0::LibraAccount;
     use 0x0::LibraSystem;
-    use 0x0::AddressUtil;
     use 0x0::Transaction;
-    use 0x0::Vector;
 
     ///////////////////////////////////////////////////////////////////////////
     // Transaction Fee Distribution
@@ -49,12 +47,12 @@ module TransactionFee {
         });
     }
 
-    public fun distribute_transaction_fees() acquires TransactionFees {
+    public fun distribute_transaction_fees<Token>() acquires TransactionFees {
       // Can only be invoked by LibraVM privilege.
       Transaction::assert(Transaction::sender() == 0x0, 33);
 
       let num_validators = LibraSystem::validator_set_size();
-      let amount_collected = LibraAccount::balance(0xFEE);
+      let amount_collected = LibraAccount::balance<Token>(0xFEE);
 
       // If amount_collected == 0, this will also return early
       if (amount_collected < num_validators) return ();
@@ -66,7 +64,7 @@ module TransactionFee {
       );
 
       // Iterate through the validators distributing fees equally
-      distribute_transaction_fees_internal(
+      distribute_transaction_fees_internal<Token>(
           amount_to_distribute_per_validator,
           num_validators,
       );
@@ -77,7 +75,7 @@ module TransactionFee {
     // any remainder (in the case that the number of validators does not
     // evenly divide the transaction fee pot) is distributed to the first
     // validator.
-    fun distribute_transaction_fees_internal(
+    fun distribute_transaction_fees_internal<Token>(
         amount_to_distribute_per_validator: u64,
         num_validators: u64
     ) acquires TransactionFees {
@@ -90,13 +88,12 @@ module TransactionFee {
             // Increment the index into the validator set.
             index = index + 1;
 
-            LibraAccount::pay_from_capability(
+            LibraAccount::pay_from_capability<Token>(
                 addr,
-                Vector::empty(),
+                x"",
                 &distribution_resource.fee_withdrawal_capability,
                 amount_to_distribute_per_validator,
-                // FIXME: Update this once we have bytearray literals
-                AddressUtil::address_to_bytes(0xFEE),
+                x"",
             );
            }
     }
