language/move-prover/tests/sources/stdlib/modules/validator_config.move
@@ -1,4 +1,5 @@
 // dep: tests/sources/stdlib/modules/transaction.move
+
 address 0x0:
 
 module ValidatorConfig {
