language/move-prover/bytecode-to-boogie/test_mvir/verify-stdlib/bytearray_util.prover.bpl
@@ -1,6 +1,0 @@
-// Native functions and helpers for bytearray_util
-
-// TODO: fill in implementation
-procedure {:inline 1} BytearrayUtil_bytearray_concat (arg0: Value, arg1: Value) returns (ret0: Value);
-requires ExistsTxnSenderAccount(__m, __txn);
-ensures old(b#Boolean(Boolean(true))) ==> !__abort_flag;
