language/move-prover/bytecode-to-boogie/test_mvir/verify-stdlib/u64_util.prover.bpl
@@ -1,6 +1,0 @@
-// Native functions and helpers for u64_util
-
-// TODO: fill in implementation
-procedure {:inline 1} U64Util_u64_to_bytes (arg0: Value) returns (ret0: Value);
-requires ExistsTxnSenderAccount(__m, __txn);
-ensures old(b#Boolean(Boolean(true))) ==> !__abort_flag;
