language/move-prover/tests/README.md
@@ -1,0 +1,21 @@
+# Tests for Move Prover
+
+This directory contains the tests for Move Prover (or Prover for short). More specifically, `sources/stdlib/modules/` contains the clones of the current Move standard modules. `sources/` contains various Move functions (with specifications) to test Prover. The functions are grouped into different `.move` files in the directory, and further grouped into sections within a file divided by the dashed comment line (e.g., `----`). Please see `source/arithm.move` for example.
+
+There is a convention for test cases under this directory. First of all, all functions defined as test cases should be valid, passing the syntax & type check. In addition, there are two kinds of test cases, which can be mixed in a file. The first type of test cases are "correct" Move functions (expected to be proved by Prover). Another type of test cases are incorrect Move functions (expected to be disproved by Prover). The incorrect functions have suffix `_incorrect` in their names for indication (this indication is currently for humans, not for automated testing tools).
+
+`cargo test` will automatically detect all `.move` files under this directory and let Prover attempt to prove each file, i.e., every function defeind in the file. Unlike `cargo run`, `cargo test` can also detect the line `// dep: {file_to_import}` in the `.move` file under test, and import other `.move` files accordingly. For each `.move` file, there is a corresponding baseline flie (`.exp`) which stores the expected Prover's output for the `.move` file. `cargo test` invokes Prover against each `.move` file, and examine the output. The test is considered to fail if the output of Prover is different from the expected output stored in the corresponding `.exp` file. To update the baseline file, run the test setting the env variable `UPBL` with 1 (i.e., `UPBL=1 cargo test`). Also, one can run the indivisual test with a specific filename (for example, `cargo test arithm.move`, `UPBL=1 cargo test arithm.move`). Note that Prover currently skips proving some functions such as the native functions and the functions in stanard vector module (`sources/stdlib/modules/vector.move`) even though these functions come with specifications.
+
+Lastly, if the environment variables such as `BOOGIE_EXE` and `Z3_EXE` are not defined, `cargo test` will only partially test Prover without invoking Boogie (e.g., only testing the translation to Boogie). The instruction for the environment variables can be found in `../scripts/README.md`.
+
+
+## Code coverage
+
+Analyzing the test coverage of the libra repo is regularly done in CI, and the result updates the online report at
+* https://codecov.io/gh/libra/libra
+
+Note that this report is based on the the coverage test when the environment variable `BOOGIE_EXE` is not set. So, the coverage result may not be as accurate as expected because all verifications with Boogie/Z3 are skipped during the test.
+
+To run the coverage test locally, one can use `scripts/coverage_report.sh`. However, note that there seems to be a small accuracy issue here too because some coverage lines are spilled in `lcov` conversion from `grcov`.
+
+For any questions regarding code coverage, please use the Calibra slack channel "#code_coverage".
